PREFIX : <https://linked.data.gov.au/def/gn-statuses/>
PREFIX agldwgstatus: <https://linked.data.gov.au/def/reg-statuses/>
PREFIX cs: <https://linked.data.gov.au/def/gn-statuses>
PREFIX dcterms: <http://purl.org/dc/terms/>
PREFIX droles: <https://linked.data.gov.au/def/data-roles/>
PREFIX owl: <http://www.w3.org/2002/07/owl#>
PREFIX prov: <http://www.w3.org/ns/prov#>
PREFIX rdfs: <http://www.w3.org/2000/01/rdf-schema#>
PREFIX reg: <http://purl.org/linked-data/registry#>
PREFIX sdo: <https://schema.org/>
PREFIX skos: <http://www.w3.org/2004/02/skos/core#>
PREFIX themes: <https://linked.data.gov.au/def/fsdf/themes/>
PREFIX xsd: <http://www.w3.org/2001/XMLSchema#>

:gazetted
    a skos:Concept ;
    rdfs:isDefinedBy cs: ;
    skos:broader :official ;
    skos:definition "The name is official and authorised in a jurisdictional gazette"@en ;
    skos:historyNote "Taken from the Place Names Ontology but with a definition added here" ;
    skos:inScheme cs: ;
    skos:prefLabel "Gazetted"@en ;
.

:published
    a skos:Concept ;
    rdfs:isDefinedBy cs: ;
    skos:broader :official ;
    skos:definition "The name is official and listed in publications"@en ;
    skos:historyNote "Taken from the Place Names Ontology but with a definition added here" ;
    skos:inScheme cs: ;
    skos:prefLabel "Published"@en ;
.

:released
    a skos:Concept ;
    rdfs:isDefinedBy cs: ;
    skos:broader :official ;
    skos:definition "The name is official but is no longer to be used and the name is available for other use"@en ;
    skos:historyNote "Taken from the Place Names Ontology but with a definition added here" ;
    skos:inScheme cs: ;
    skos:prefLabel "Released"@en ;
.

:retired
    a skos:Concept ;
    rdfs:isDefinedBy cs: ;
    skos:broader :official ;
    skos:definition "The name is official but is now no longer to be used"@en ;
    skos:historyNote "Taken from the Place Names Ontology but with a definition added here" ;
    skos:inScheme cs: ;
    skos:prefLabel "Retired"@en ;
.

:historical
    a skos:Concept ;
    rdfs:isDefinedBy cs: ;
    skos:definition "The name has been used historically and perhaps currently but is not an official name"@en ;
    skos:historyNote "Taken from the Place Names Ontology but with a definition added here" ;
    skos:inScheme cs: ;
    skos:prefLabel "Historical"@en ;
    skos:topConceptOf cs: ;
.

:indigenous
    a skos:Concept ;
    rdfs:isDefinedBy cs: ;
    skos:definition "The name is used by indigenous communities"@en ;
    skos:historyNote "New in this vocabulary" ;
    skos:inScheme cs: ;
    skos:prefLabel "Indigenous"@en ;
    skos:topConceptOf cs: ;
.

:informal
    a skos:Concept ;
    rdfs:isDefinedBy cs: ;
    skos:definition "The name is used but it is not official"@en ;
    skos:historyNote "Taken from the Place Names Ontology but with a definition added here" ;
    skos:inScheme cs: ;
    skos:narrower
        :historical ,
        :indigenous ;
    skos:prefLabel "Informal"@en ;
    skos:topConceptOf cs: ;
.

:official
    a skos:Concept ;
    rdfs:isDefinedBy cs: ;
    skos:definition "The name has been sanctioned by an authoritative institution"@en ;
    skos:historyNote "Taken from the Place Names Ontology but with a definition added here" ;
    skos:inScheme cs: ;
    skos:narrower
        :gazetted ,
        :published ,
        :released ,
        :retired ;
    skos:prefLabel "Official"@en ;
    skos:topConceptOf cs: ;
.

<https://linked.data.gov.au/org/qsi>
    a sdo:Organization ;
    sdo:name "Queensland Spatial Information" ;
    sdo:url "https://www.resources.qld.gov.au/data-mapping"^^xsd:anyURI ;
.

<https://linked.data.gov.au/org/icsm>
    a sdo:Organization ;
    sdo:name "Intergovernmental Committee on Surveying & Mapping" ;
    sdo:url "https://icsm.gov.au"^^xsd:anyURI ;
.

cs:
    a skos:ConceptScheme ;
    sdo:keywords themes:place-names ;
    dcterms:created "2023-06-12"^^xsd:date ;
    dcterms:creator <https://linked.data.gov.au/org/qsi> ;
    dcterms:modified "2023-11-30"^^xsd:date ;
    dcterms:publisher <https://linked.data.gov.au/org/icsm> ;
    reg:status agldwgstatus:experimental ;
    owl:versionIRI :1.0 ;
    owl:versionInfo "1.0" ;
    skos:definition "This vocabulary contains classifications of how official, or otherwise, a Geographical Name is"@en ;
    skos:hasTopConcept
        :indigenous ,
        :informal ,
        :official ;
    skos:historyNote "Taken from the Place Names Ontology (https://linked.data.gov.au/def/placenames)"@en ;
    skos:prefLabel "Geographical Name Statuses"@en ;
    skos:scopeNote "These statuses do not indicate whether a Geographical Name is current. Currency of Geographical Names should be indicated by temporal properties" ;
    prov:qualifiedAttribution
        [
            prov:hadRole droles:custodian ;
            prov:agent <https://linked.data.gov.au/org/icsm>
        ] ;
.

