PREFIX agldwgstatus: <https://linked.data.gov.au/def/reg-statuses/>
PREFIX cs: <http://linked.data.gov.au/def/survey-type>
PREFIX dcterms: <http://purl.org/dc/terms/>
PREFIX owl: <http://www.w3.org/2002/07/owl#>
PREFIX rdfs: <http://www.w3.org/2000/01/rdf-schema#>
PREFIX reg: <http://purl.org/linked-data/registry#>
PREFIX sdo: <https://schema.org/>
PREFIX skos: <http://www.w3.org/2004/02/skos/core#>
PREFIX svytp: <http://linked.data.gov.au/def/survey-type/>
PREFIX xsd: <http://www.w3.org/2001/XMLSchema#>

svytp:atmospheric
    a skos:Concept ;
    skos:historyNote "Compiled by the Geological Survey of Queensland" ;
    rdfs:isDefinedBy cs: ;
    skos:definition "A survey measuring chemical and physical properties of the atmosphere."@en ;
    skos:inScheme cs: ;
    skos:notation "at" ;
    skos:prefLabel "Atmospheric"@en ;
    skos:topConceptOf cs: ;
.

svytp:geochemistry
    a skos:Concept ;
    skos:historyNote "Compiled by the Geological Survey of Queensland" ;
    rdfs:isDefinedBy cs: ;
    skos:definition "A survey where the chemical properties of rocks, soil, or other geological material is assessed to determine mineralogical and/or elemental composition."@en ;
    skos:inScheme cs: ;
    skos:notation "gc" ;
    skos:prefLabel "Geochemistry"@en ;
    skos:topConceptOf cs: ;
.

svytp:geophysical
    a skos:Concept ;
    skos:historyNote "Compiled by the Geological Survey of Queensland" ;
    rdfs:isDefinedBy cs: ;
    skos:definition "A survey where the geophysical properties of the earth is assessed."@en ;
    skos:inScheme cs: ;
    skos:notation "gp" ;
    skos:prefLabel "Geophysical"@en ;
    skos:topConceptOf cs: ;
.

svytp:geotechnical
    a skos:Concept ;
    skos:historyNote "Compiled by the Geological Survey of Queensland" ;
    rdfs:isDefinedBy cs: ;
    skos:altLabel "Geomechanical"@en ;
    skos:definition "A survey measuring the physical and mechanical properties of rocks, soil and earth material with particular focus on rock strength and competence."@en ;
    skos:inScheme cs: ;
    skos:notation "gt" ;
    skos:prefLabel "Geotechnical"@en ;
    skos:topConceptOf cs: ;
.

svytp:hydrochemistry
    a skos:Concept ;
    skos:historyNote "Compiled by the Geological Survey of Queensland" ;
    rdfs:isDefinedBy cs: ;
    skos:definition "A survey of the chemical and physical properties of surface or ground water."@en ;
    skos:inScheme cs: ;
    skos:notation "hy" ;
    skos:prefLabel "Hydrochemistry"@en ;
    skos:topConceptOf cs: ;
.

svytp:petrophysical
    a skos:Concept ;
    skos:historyNote "Compiled by the Geological Survey of Queensland" ;
    rdfs:isDefinedBy cs: ;
    skos:definition "A survey that records physical, chemical, electrical, or other properties of the rock/fluid mixtures. This may appliy to measurements derived via wireline logging, or properties analysed in a laboratory setting."@en ;
    skos:inScheme cs: ;
    skos:notation "py" ;
    skos:prefLabel "Petrophysical"@en ;
    skos:topConceptOf cs: ;
.

svytp:physical-geology
    a skos:Concept ;
    skos:historyNote "Compiled by the Geological Survey of Queensland" ;
    rdfs:isDefinedBy cs: ;
    skos:altLabel "Field Mapping"@en ;
    skos:definition "A survey of physical geological features such as outcrop samples, structural measurements, sedimentological and stratigraphic observations."@en ;
    skos:inScheme cs: ;
    skos:notation "pg" ;
    skos:prefLabel "Physical Geology"@en ;
    skos:topConceptOf cs: ;
.

svytp:resource-extractives
    a skos:Concept ;
    skos:historyNote "Compiled by the Geological Survey of Queensland" ;
    rdfs:isDefinedBy cs: ;
    skos:definition "A survey capturing both production and sales statistics for a quarry in a given period."@en ;
    skos:inScheme cs: ;
    skos:notation "re" ;
    skos:prefLabel "Resource Extractives"@en ;
    skos:topConceptOf cs: ;
.

svytp:resource-reserves
    a skos:Concept ;
    skos:historyNote "Compiled by the Geological Survey of Queensland" ;
    rdfs:isDefinedBy cs: ;
    skos:definition "A survey capturing the resources and reserves statistics in a given period."@en ;
    skos:inScheme cs: ;
    skos:notation "rp" ;
    skos:prefLabel "Resources and Reserves"@en ;
    skos:topConceptOf cs: ;

svytp:resource-production
    a skos:Concept ;
    skos:historyNote "Compiled by the Geological Survey of Queensland" ;
    rdfs:isDefinedBy cs: ;
    skos:definition "A survey capturing the production and processing statistics of a mine site in a given period."@en ;
    skos:inScheme cs: ;
    skos:notation "rp" ;
    skos:prefLabel "Resource Production"@en ;
    skos:topConceptOf cs: ;
.

svytp:resource-sales
    a skos:Concept ;
    skos:historyNote "Compiled by the Geological Survey of Queensland" ;
    rdfs:isDefinedBy cs: ;
    skos:definition "A survey capturing the sales statistics of a mine site in a given period."@en ;
    skos:inScheme cs: ;
    skos:notation "rs" ;
    skos:prefLabel "Resource Sales"@en ;
    skos:topConceptOf cs: ;
.

svytp:seismic
    a skos:Concept ;
    skos:historyNote "Compiled by the Geological Survey of Queensland" ;
    rdfs:isDefinedBy cs: ;
    skos:definition "A survey using the interaction of seismic waves with sub-surface features of the earth to determine properties and morphology of those features."@en ;
    skos:inScheme cs: ;
    skos:notation "ss" ;
    skos:prefLabel "Seismic"@en ;
    skos:topConceptOf cs: ;
.

svytp:spatial
    a skos:Concept ;
    skos:historyNote "Compiled by the Geological Survey of Queensland" ;
    rdfs:isDefinedBy cs: ;
    skos:altLabel "Location Survey"@en ;
    skos:definition "A survey measuring the spatial characteristics of an object or region."@en ;
    skos:inScheme cs: ;
    skos:notation "st" ;
    skos:prefLabel "Spatial"@en ;
    skos:topConceptOf cs: ;
.

svytp:spectral
    a skos:Concept ;
    skos:historyNote "Compiled by the Geological Survey of Queensland" ;
    rdfs:isDefinedBy cs: ;
    skos:definition "A survey capturing image information and intensity-per-wavelength-band to be used for spectral analysis e.g. ASTER, MODIS."@en ;
    skos:inScheme cs: ;
    skos:notation "sp" ;
    skos:prefLabel "Spectral"@en ;
    skos:topConceptOf cs: ;
.

<https://linked.data.gov.au/org/gsq>
    a sdo:Organization ;
    sdo:name "Geological Survey of Queensland" ;
    sdo:url "http://www.business.qld.gov.au/industries/mining-energy-water/resources/geoscience-information/gsq"^^xsd:anyURI ;
.

cs:
    a
        owl:Ontology ,
        skos:ConceptScheme ;
    dcterms:created "2020-02-05"^^xsd:date ;
    dcterms:creator <https://linked.data.gov.au/org/gsq> ;
    dcterms:modified "2023-03-16"^^xsd:date ;
    skos:historyNote "Compiled by the Geological Survey of Queensland" ;
    dcterms:publisher <https://linked.data.gov.au/org/gsq> ;
    reg:status agldwgstatus:stable ;
    skos:definition "The one-off event examining a geological or administrative feature. The type of survey or sampling performed to investigate a feature, site, or sample. Surveys are activities that produce samples or make one-or-many observations."@en ;
    skos:hasTopConcept
        svytp:atmospheric ,
        svytp:geochemistry ,
        svytp:geophysical ,
        svytp:geotechnical ,
        svytp:hydrochemistry ,
        svytp:petrophysical ,
        svytp:physical-geology ,
        svytp:resource-extractives ,
        svytp:resource-production ,
        svytp:resource-sales ,
        svytp:seismic ,
        svytp:spatial ,
        svytp:spectral ;
    skos:prefLabel "Survey Type"@en ;
.

